Add %~ syntax for approximates (on scalars, sequences)

src/lib/kuiper/Kuiper.Approximates.fsti
@@ -1,6 +1,6 @@
 module Kuiper.Approximates
 
-include Kuiper.Approximates.Class
+include Kuiper.Approximates.Base
 
 include Kuiper.Approximates.U8
 include Kuiper.Approximates.U16
@@ -15,10 +15,29 @@ open FStar.Real
 open Kuiper.Scalars
 open Kuiper.Seq.Common
 
+(* This class provides some syntactic sugar to use the ~~ operator
+   on scalars, sequences, matrices, etc. *)
+class can_approximate (c m : Type) = {
+  approximates : c -> m -> prop;
+}
+
+unfold let (%~) #c #m (x:c) (y:m) {| can_approximate c m |}
+  : prop = approximates x y
+
+instance real_like_can_approximate (#a:Type) (_ : scalar a) (_ : real_like a)
+  : can_approximate a Real.real = {
+  approximates = v_approximates;
+}
+
 let seq_approximates (#a:Type) {| scalar a, real_like a |}
   (s : seq a) (r : seq Real.real) : prop
   = Seq.length s == Seq.length r /\
-    (forall i. i < len s ==> (s @! i) `approximates` (r @! i))
+    (forall i. i < len s ==> (s @! i) %~ (r @! i))
+
+instance seq_real_like_can_approximate (#a:Type) {| scalar a, real_like a |}
+  : can_approximate (seq a) (seq Real.real) = {
+  approximates = seq_approximates;
+}
 
 let to_real_seq (#a:Type) {| scalar a, real_like a |}
   (s : seq a) : GTot (seq Real.real)
@@ -26,7 +45,7 @@ let to_real_seq (#a:Type) {| scalar a, real_like a |}
 
 val to_real_seq_is_approx (#a:Type) {| scalar a, real_like a |}
   (s : seq a)
-  : Lemma (seq_approximates s (to_real_seq s))
+  : Lemma (s %~ to_real_seq s)
           [SMTPat (seq_approximates s (to_real_seq s))]
 
 let real_seq_sum (r : seq Real.real) : Real.real
@@ -38,5 +57,5 @@ val real_seq_sum_append
 
 val seq_approximates_append (#a:Type) {| scalar a, real_like a |}
   (s1 s2 : a) (r1 r2 : seq Real.real)
-  : Lemma (requires s1 `approximates` real_seq_sum r1 /\ s2 `approximates` real_seq_sum r2)
-          (ensures (s1 `add` s2) `approximates` real_seq_sum (r1 `Seq.append` r2))
+  : Lemma (requires s1 %~ real_seq_sum r1 /\ s2 %~ real_seq_sum r2)
+          (ensures (s1 `add` s2) %~ real_seq_sum (r1 `Seq.append` r2))
