src/lib/kuiper/Kuiper.Approximates.F64.fsti
@@ -1,6 +1,6 @@
 module Kuiper.Approximates.F64
 
 open Kuiper
-open Kuiper.Approximates.Class
+open Kuiper.Approximates.Base
 
 instance val real_like_f64 : real_like f64
