src/lib/kuiper/Kuiper.Approximates.U32.fsti
@@ -1,6 +1,6 @@
 module Kuiper.Approximates.U32
 
 open Kuiper
-open Kuiper.Approximates.Class
+open Kuiper.Approximates.Base
 
 instance val real_like_u32 : real_like u32
